progress

sat.dfy
@@ -4,7 +4,44 @@ include "util.dfy"
 // inspired by https://siddhartha-gadgil.github.io/automating-mathematics/posts/sat-solving/
 newtype Variable = int
 
-datatype Exp =
+
+lemma demorgan1(s: set<Expression>, vs: map<Variable,bool>)
+    requires |s| >= 1
+    requires forall i :: i in s ==> i.Valid()
+    requires forall i :: i in s ==> vs.Keys >= i.all_vars()
+    ensures 
+        Not(Or(s)).eval(vs) == 
+        And(map_not_empty(s, map i | i in s :: Not(i))).eval(vs)
+{
+    var x := Not(Or(s)).eval(vs);
+    var or := Or(s);
+    assert or.eval(vs) == (!forall i :: i in s ==> !i.eval(vs));
+    assert x == !(!forall i :: i in s ==> !i.eval(vs));
+
+    var nots := map_not_empty(s, map i | i in s :: Not(i));
+    var y := And(nots).eval(vs);
+    assert And(nots).eval(vs) == (forall i :: i in nots ==> i.eval(vs));
+    assert !(!forall i :: i in s ==> !i.eval(vs)) == (forall i :: i in s ==> Not(i).eval(vs));
+}
+
+lemma demorgan2(s: set<Expression>, vs: map<Variable,bool>)
+    requires |s| >= 1
+    requires forall i :: i in s ==> i.Valid() && vs.Keys >= i.all_vars()
+    ensures Not(And(s)).eval(vs) == Or(map_not_empty(s, map i | i in s :: Not(i))).eval(vs)
+{
+    var and := And(s);
+    var x := Not(and).eval(vs);
+    assert and.eval(vs) != x;
+    assert and.eval(vs) == forall i :: i in s ==> i.eval(vs);
+    assert and.eval(vs) == !(exists i :: i in s && !i.eval(vs));
+    assert x == exists i :: i in s && !i.eval(vs);
+
+    var nots := map_not_empty(s, map i | i in s :: Not(i));
+    var y := Or(nots).eval(vs);
+    assert Or(nots).eval(vs) == exists n :: n in nots && n.eval(vs);
+}
+
+datatype Expression =
     Constant(bool) |
     Var(Variable) |
     Not(Expression) |
@@ -39,74 +76,46 @@ datatype Exp =
         }
     }
 
-    // function vars() : (vs: set<Variable>)
-    //     requires this.Valid()
-    //     decreases this.height
-    //     ensures forall i :: i in this.exp.children() ==> vs >= i.vars()
-    // {
-    //     match exp {
-    //         case Constant(b) => {}
-    //         case Var(v) => {v}
-    //         case Not(e) => e.vars()
-    //         case And(ands) => flatten(set a | a in ands :: a.vars())
-    //         case Or(ors) => flatten(set o | o in ors :: o.vars())
-    //         case Implies(a,b) => a.vars() + b.vars()
-    //         case Equivalent(a,b) => a.vars() + b.vars()
-    //     }
-    // }
+    predicate Valid()
+    {
+        LocalValid() &&
+        forall i :: i in children() ==> i.LocalValid() && i.Valid()
+    }
 
-    function height() : int
-        requires LocalValid()
+    function self_vars() : (vs: set<Variable>)
     {
         match this {
-            case Constant(b) => 0
-            case Var(v) => 0
-            case Not(e) => e.height + 1
-            case And(ands) =>
-                var heights := map_set(ands, (i: Expression) => i.exp.height());
-                max(heights) + 1
-            case Or(ors) => max(set i | i in ors :: i.height) + 1
-            case Implies(a,b) => max({a.height, b.height}) + 1
-            case Equivalent(a,b) => max({a.height, b.height}) + 1
+            case Var(v) => {v}
+            case _ => {}
         }
     }
-}
 
-function make_exp(exp: Exp) : (e: Expression)
-    requires forall c :: c in exp.children() ==> c.Valid()
-    ensures e.Valid()
-{
-    var h := if |exp.children()| == 0 then
-        0
-    else
-        var heights_set := map_set(exp.children(), (c: Expression) => c.height);
-        var max_child := max(heights_set);
-        max_child + 1;
-    Expression(h, exp)
-}
-
-datatype Expression = Expression(height: int, exp: Exp)
-{
-    ghost predicate Valid()
-        decreases this.height
+    function all_vars() : (vs: set<Variable>)
+        requires this.Valid()
+        decreases this
+        ensures forall v :: true ==> (v in vs <==> v in self_vars() || exists c :: c in children() && v in c.all_vars())
     {
-        this.height >= 0 &&
-        if this.height == 0 then
-            |this.exp.children()| == 0
-        else
-            forall c :: c in this.exp.children() ==>
-                this.height > c.height &&
-                c.Valid()
-    }
- 
+        var vs := flatten(match this {
+            case Constant(b) => {{}}
+            case Var(vv) => {{vv}}
+            case Not(e) => {e.all_vars()}
+            case And(ands) => set a | a in ands :: a.all_vars()
+            case Or(ors) => set o | o in ors :: o.all_vars()
+            case Implies(a,b) => {a.all_vars(), b.all_vars()}
+            case Equivalent(a,b) => {a.all_vars(), b.all_vars()}
+        });
 
+        assert forall v :: true ==> (v in vs <==> v in self_vars() || exists c :: c in children() && v in c.all_vars());
+
+        vs
+    }
 
     function eval(vs: map<Variable,bool>) : bool
         requires this.Valid()
-        requires vs.Keys >= this.vars()
-        decreases this.height
+        requires vs.Keys >= this.all_vars()
+        decreases this
     {
-        match exp {
+        match this {
             case Constant(b) => b
             case Var(v) => vs[v]
             case Not(e) => !e.eval(vs)
@@ -117,424 +126,402 @@ datatype Expression = Expression(height: int, exp: Exp)
         }
     }
 
- 
-
-    // lemma descendent_vars(e: Expression, vs: set<Variable>)
-    //     requires e.vars() == vs
-    //     decreases e.height
-    //     //ensures forall i :: i in descendents(e) ==> vars(e) >= vars(i)
-    // {
-    //     assert forall i :: i in e.exp.children() ==> e.vars() >= i.vars();
-    //     var cs := e.exp.children();
-    //     var cds := flatten(set i | i in e.exp.children() :: i.descendents());
-    //     var ds := e.descendents();
-    //     //assert cds < ds;
-
-    //     var cds_vs := set_vars(cds);
-    //     var ds_vs := set_vars(ds);
-    // }
-
-    function descendents() : (d: set<Expression>)
-        requires this.Valid()
-        decreases this.exp
-        ensures this.exp.children() <= d
-        ensures forall i :: i in d ==> this.height > i.height
-        ensures forall i :: i in this.exp.children() ==> descendents() < d
-    {
-        match exp {
-            case Constant(b) => {}
-            case Var(v) => {}
-            case Not(x) => {x} + x.descendents()
-            case And(s) => s + flatten(set i | i in s :: i.descendents())
-            case Or(s) => s + flatten(set i | i in s :: i.descendents())
-            case Implies(a,b) => {a, b} + a.descendents() + b.descendents()
-            case Equivalent(a,b) => {a, b} + a.descendents() + b.descendents()
-        }
-    }
-
     function simplify_one(vs: map<Variable,bool>) : (out: Expression)
-        requires vs.Keys >= this.vars()
+        requires this.Valid()
+        requires vs.Keys >= this.all_vars()
         decreases this
-        ensures match out.exp {
+        ensures out.Valid()
+        ensures match out {
             case Implies(_,_) => false
             case Equivalent(_,_) => false
             case Not(ee) =>
-                match ee.exp {
+                match ee {
                     case Or(_) => false
                     case And(_) => false
                     case _ => true
                 }
             case e => true
         }
-        ensures this.vars() >= out.vars()
+        ensures this.all_vars() >= out.all_vars()
         ensures this.eval(vs) == out.eval(vs)
     {
-        match this.exp {
-            case Implies(a,b) => make_exp(Or({make_exp(Not(a)), b}))
+        match this {
+            case Implies(a,b) => 
+                var out := Or({Not(a), b});
+                assert out.all_vars() <= this.all_vars();
+                assert this.eval(vs) == out.eval(vs);
+                out
             case Equivalent(a,b) =>
-                var both_true := make_exp(And({a,b}));
+                var both_true := And({a,b});
                 assert both_true.eval(vs) == (a.eval(vs) && b.eval(vs));
-                var first_false := make_exp(Not(a));
-                var second_false := make_exp(Not(b));
-                var both_false := make_exp(And({first_false, second_false}));
-                assert both_false.vars() <= this.vars();
+                var first_false := Not(a);
+                var second_false := Not(b);
+                var both_false := And({first_false, second_false});
+                assert both_false.all_vars() <= this.all_vars();
                 assert both_false.eval(vs) == (!a.eval(vs) && !b.eval(vs));
-                var out := make_exp(Or({both_true, both_false}));
-                assert out.vars() <= this.vars();
+                var out := Or({both_true, both_false});
+                assert out.all_vars() <= this.all_vars();
                 assert this.eval(vs) == out.eval(vs);
                 out
             case Not(n) =>
-                var out := make_exp(match n.exp {
+                assert n.Valid();
+                var out := match n {
                     case Or(s) =>
                         // n.exp.descendents_vars(vs);
-                        s.demorgan1(vs);
-                        make_exp(And(set i | i in s :: Not(i)))
+                        demorgan1(s, vs);
+                        And(map_not_empty(s, map i | i in s :: Not(i)))
                     case And(s) =>
                         // n.exp.descendents_vars(vs);
-                        s.demorgan2(vs);
-                        make_exp(Or(set i | i in s :: Not(i)))
+                        demorgan2(s, vs);
+                        Or(map_not_empty(s, map i | i in s :: Not(i)))
                     case _ => this
-                });
+                };
+                assert this.all_vars() >= out.all_vars();
                 assert this.eval(vs) == out.eval(vs);
                 out
             case e => e
         }
     }
-
-    lemma demorgan1(s: set<Exp>, vs: map<Variable,bool>)
-        requires forall i :: i in s ==> vs.Keys >= i.vars()
-        ensures 
-            make_exp(Not(make_exp(Or(s)))).eval(vs) == 
-            make_exp(And(set i | i in s :: make_exp(Not(i)))).eval(vs)
-    {
-        var x := make_exp(Not(make_exp(Or(s)))).eval(vs);
-        var or := make_exp(Or(s));
-        assert or.eval(vs) == (!forall i :: i in s ==> !i.eval(vs));
-        assert x == !(!forall i :: i in s ==> !i.eval(vs));
-
-        var y := make_exp(And(set i | i in s :: make_exp(Not(i)))).eval(vs);
-        var nots := set i | i in s :: make_exp(Not(i));
-        assert y == make_exp(And(nots)).eval(vs);
-        assert make_exp(And(nots)).eval(vs) == (forall i :: i in nots ==> i.eval(vs));
-        assert !(!forall i :: i in s ==> !i.eval(vs)) == (forall i :: i in s ==> make_exp(Not(i)).eval(vs));
-    }
 }
 
 
 
-// function child_descendents(e: Expression) : (cd_flat: set<Expression>)
-//     ensures flatten(set i | i in children(e) :: descendents(i)) <= descendents(e)
-//     ensures cd_flat == flatten(set i | i in children(e) :: descendents(i))
-// {
-//     child_descendents_helper(e, descendents(e))
+
+ 
+
+//     // lemma descendent_vars(e: Expression, vs: set<Variable>)
+//     //     requires e.vars() == vs
+//     //     decreases e.height
+//     //     //ensures forall i :: i in descendents(e) ==> vars(e) >= vars(i)
+//     // {
+//     //     assert forall i :: i in e.exp.children() ==> e.vars() >= i.vars();
+//     //     var cs := e.exp.children();
+//     //     var cds := flatten(set i | i in e.exp.children() :: i.descendents());
+//     //     var ds := e.descendents();
+//     //     //assert cds < ds;
+
+//     //     var cds_vs := set_vars(cds);
+//     //     var ds_vs := set_vars(ds);
+//     // }
+
+//     function descendents() : (d: set<Expression>)
+//         requires this.Valid()
+//         decreases this.exp
+//         ensures this.exp.children() <= d
+//         ensures forall i :: i in d ==> this.height > i.height
+//         ensures forall i :: i in this.exp.children() ==> descendents() < d
+//     {
+//         match exp {
+//             case Constant(b) => {}
+//             case Var(v) => {}
+//             case Not(x) => {x} + x.descendents()
+//             case And(s) => s + flatten(set i | i in s :: i.descendents())
+//             case Or(s) => s + flatten(set i | i in s :: i.descendents())
+//             case Implies(a,b) => {a, b} + a.descendents() + b.descendents()
+//             case Equivalent(a,b) => {a, b} + a.descendents() + b.descendents()
+//         }
+//     }
+
+
 // }
 
-// function child_descendents_helper(e: Expression, d: set<Expression>) : (cd_flat: set<Expression>)
-//     requires d == descendents(e)
-//     ensures flatten(set i | i in children(e) :: descendents(i)) <= d
-//     ensures cd_flat == flatten(set i | i in children(e) :: descendents(i))
-// {
-//     assert forall i :: i in children(e) ==> descendents(i) < d;
-//     assert e !in d;
 
-//     var cs := children(e);
-//     assert forall i :: i in cs ==> descendents(i) < d;
-//     assert cs == children(e);
-//     var cd_flat := flatten(set i | i in cs :: descendents(i));
-//     assert cd_flat == flatten(set i | i in children(e) :: descendents(i));
-//     assert cd_flat + cs == d;
-//     assert cd_flat <= d;
-//     cd_flat
+
+// // function child_descendents(e: Expression) : (cd_flat: set<Expression>)
+// //     ensures flatten(set i | i in children(e) :: descendents(i)) <= descendents(e)
+// //     ensures cd_flat == flatten(set i | i in children(e) :: descendents(i))
+// // {
+// //     child_descendents_helper(e, descendents(e))
+// // }
+
+// // function child_descendents_helper(e: Expression, d: set<Expression>) : (cd_flat: set<Expression>)
+// //     requires d == descendents(e)
+// //     ensures flatten(set i | i in children(e) :: descendents(i)) <= d
+// //     ensures cd_flat == flatten(set i | i in children(e) :: descendents(i))
+// // {
+// //     assert forall i :: i in children(e) ==> descendents(i) < d;
+// //     assert e !in d;
+
+// //     var cs := children(e);
+// //     assert forall i :: i in cs ==> descendents(i) < d;
+// //     assert cs == children(e);
+// //     var cd_flat := flatten(set i | i in cs :: descendents(i));
+// //     assert cd_flat == flatten(set i | i in children(e) :: descendents(i));
+// //     assert cd_flat + cs == d;
+// //     assert cd_flat <= d;
+// //     cd_flat
+// // }
+
+// // function height(e: Expression) : (h: int)
+// //     decreases e
+// //     ensures h >= 0
+// //     ensures forall i :: i in children(e) ==> h > height(i)
+// // {
+// //     match e {
+// //         case Constant(b) => 0
+// //         case Var(v) => 0
+// //         case Not(e) => height(e) + 1
+// //         case And(s) =>
+// //             if |s| == 0 then
+// //                 0
+// //             else
+// //                 assert s == children(e);
+// //                 var heights_set := set i | i in s :: height(i);
+// //                 var heights_map := map i | i in s :: height(i);
+// //                 assert forall i :: i in s ==> height(i) in heights_set;
+// //                 assert forall i :: i in s ==> i in heights_map.Keys;
+// //                 assert forall i :: i in s ==> height(i) in heights_map.Values;
+// //                 assert heights_set == heights_map.Values;
+// //                 notempty(s, heights_map);
+// //                 var max_child := max(heights_set);
+// //                 var h := max_child + 1;
+// //                 assert forall i :: i in children(e) ==> h > height(i);
+// //                 h
+// //         case Or(s) =>
+// //             if |s| == 0 then
+// //                 0
+// //             else
+// //                 assert s == children(e);
+// //                 var heights_set := set i | i in s :: height(i);
+// //                 var heights_map := map i | i in s :: height(i);
+// //                 assert forall i :: i in s ==> height(i) in heights_set;
+// //                 assert forall i :: i in s ==> i in heights_map.Keys;
+// //                 assert forall i :: i in s ==> height(i) in heights_map.Values;
+// //                 assert heights_set == heights_map.Values;
+// //                 notempty(s, heights_map);
+// //                 var max_child := max(heights_set);
+// //                 var h := max_child + 1;
+// //                 assert forall i :: i in children(e) ==> h > height(i);
+// //                 h
+// //         case Implies(a,b) => max({height(a), height(b)}) + 1
+// //         case Equivalent(a,b) => max({height(a), height(b)}) + 1
+// //     }
+// // }
+
+
+// /*
+// function set_vars(s: set<Expression>) : (vs: set<Variable>)
+//     ensures forall i :: i in s ==> vars(i) <= vs
+//     ensures flatten(set i | i in s :: vars(i)) == vs
+// {
+//     flatten(set i | i in s :: vars(i))
 // }
 
-// function height(e: Expression) : (h: int)
-//     decreases e
-//     ensures h >= 0
-//     ensures forall i :: i in children(e) ==> h > height(i)
+// lemma bigger_set_bigger_vars(a: set<Expression>, b: set<Expression>, av: set<Variable>, bv: set<Variable>)
+//     requires a <= b
+//     requires set_vars(a) == av && set_vars(b) == bv
+//     ensures av <= bv
 // {
-//     match e {
-//         case Constant(b) => 0
-//         case Var(v) => 0
-//         case Not(e) => height(e) + 1
-//         case And(s) =>
-//             if |s| == 0 then
-//                 0
-//             else
-//                 assert s == children(e);
-//                 var heights_set := set i | i in s :: height(i);
-//                 var heights_map := map i | i in s :: height(i);
-//                 assert forall i :: i in s ==> height(i) in heights_set;
-//                 assert forall i :: i in s ==> i in heights_map.Keys;
-//                 assert forall i :: i in s ==> height(i) in heights_map.Values;
-//                 assert heights_set == heights_map.Values;
-//                 notempty(s, heights_map);
-//                 var max_child := max(heights_set);
-//                 var h := max_child + 1;
-//                 assert forall i :: i in children(e) ==> h > height(i);
-//                 h
-//         case Or(s) =>
-//             if |s| == 0 then
-//                 0
-//             else
-//                 assert s == children(e);
-//                 var heights_set := set i | i in s :: height(i);
-//                 var heights_map := map i | i in s :: height(i);
-//                 assert forall i :: i in s ==> height(i) in heights_set;
-//                 assert forall i :: i in s ==> i in heights_map.Keys;
-//                 assert forall i :: i in s ==> height(i) in heights_map.Values;
-//                 assert heights_set == heights_map.Values;
-//                 notempty(s, heights_map);
-//                 var max_child := max(heights_set);
-//                 var h := max_child + 1;
-//                 assert forall i :: i in children(e) ==> h > height(i);
-//                 h
-//         case Implies(a,b) => max({height(a), height(b)}) + 1
-//         case Equivalent(a,b) => max({height(a), height(b)}) + 1
+
+// }
+// /*
+
+
+
+// */
+
+
+
+
+
+// predicate no_implies(e: Expression) {
+//     forall i :: i in {e} + descendents(e) ==> match i {
+//         case Implies(_,_) => false
+//         case e => true
 //     }
 // }
 
+// function method simplify_implies(e: Expression, vs: map<Variable,bool>) : (out: Expression)
+//     requires vs.Keys >= vars(e)
+//     decreases e
+//     ensures no_implies(out)
+//     ensures vars(e) >= vars(out)
+//     ensures eval(e, vs) == eval(out, vs)
+// {
+//     descendents_vars(e, vs);
+//     var out := match e {
+//         case Constant(b) =>
+//             assert no_implies(e);
+//             e
+//         case Var(v) =>
+//             assert no_implies(e);
+//             e
+//         case Not(x) =>
+//             var xx := simplify_implies(x, vs);
+//             assert no_implies(xx);
+//             assert no_implies(Not(xx));
+//             Not(xx)
+//         case And(s) =>
+//             var ss := set i | i in s :: simplify_implies(i, vs);
+//             assert forall i :: i in ss ==> no_implies(i);
+//             assert no_implies(And(ss));
+//             And(ss)
+//         case Or(s) =>
+//             var ss := set i | i in s :: simplify_implies(i, vs);
+//             assert forall i :: i in ss ==> no_implies(i);
+//             assert no_implies(Or(ss));
+//             Or(ss)
+//         case Implies(a,b) =>
+//             var a:= simplify_implies(a, vs);
+//             assert no_implies(a) && no_implies(Not(a));
+//             var b := simplify_implies(b, vs);
+//             assert no_implies(b);
+//             assert no_implies(Or({Not(a), b}));
+//             Or({Not(a), b})
+//         case Equivalent(a,b) =>
+//             var a:= simplify_implies(a, vs);
+//             assert no_implies(a);
+//             var b := simplify_implies(b, vs);
+//             assert no_implies(b);
+//             assert no_implies(Equivalent(a, b));
+//             Equivalent(a, b)
+//     };
 
-/*
-function set_vars(s: set<Expression>) : (vs: set<Variable>)
-    ensures forall i :: i in s ==> vars(i) <= vs
-    ensures flatten(set i | i in s :: vars(i)) == vs
-{
-    flatten(set i | i in s :: vars(i))
-}
+//     out
+// }
 
-lemma bigger_set_bigger_vars(a: set<Expression>, b: set<Expression>, av: set<Variable>, bv: set<Variable>)
-    requires a <= b
-    requires set_vars(a) == av && set_vars(b) == bv
-    ensures av <= bv
-{
+// predicate no_equivalent(e: Expression) {
+//     forall i :: i in {e} + descendents(e) ==> match i {
+//         case Equivalent(_,_) => false
+//         case e => true
+//     }
+// }
 
-}
-/*
+// function method simplify_equivalent(e: Expression, vs: map<Variable,bool>) : (out: Expression)
+//     requires vs.Keys >= vars(e)
+//     requires no_implies(e)
+//     decreases e
+//     ensures no_equivalent(out)
+//     ensures vars(e) >= vars(out)
+//     ensures eval(e, vs) == eval(out, vs)
+// {
+//     descendents_vars(e, vs);
+//     var out := match e {
+//         case Constant(b) =>
+//             assert no_equivalent(e);
+//             e
+//         case Var(v) =>
+//             assert no_equivalent(e);
+//             e
+//         case Not(x) =>
+//             var xx := simplify_equivalent(x, vs);
+//             assert no_equivalent(xx);
+//             assert no_equivalent(Not(xx));
+//             Not(xx)
+//         case And(s) =>
+//             var ss := set i | i in s :: simplify_equivalent(i, vs);
+//             assert forall i :: i in ss ==> no_equivalent(i);
+//             assert no_equivalent(And(ss));
+//             And(ss)
+//         case Or(s) =>
+//             var ss := set i | i in s :: simplify_equivalent(i, vs);
+//             assert forall i :: i in ss ==> no_equivalent(i);
+//             assert no_equivalent(Or(ss));
+//             Or(ss)
+//         case Implies(a,b) =>
+//             assert false;
+//             a
+//         case Equivalent(a,b) =>
+//             var a:= simplify_equivalent(a, vs);
+//             assert no_equivalent(a);
+//             var b := simplify_equivalent(b, vs);
+//             assert no_equivalent(b);
+//             var out := Or(And({a,b}),And({Not(a),Not(b)}));
+//             assert no_implies(out);
+//             out
+//     };
 
+//     out
+// }
 
+// predicate no_not_expressions(e: Expression) {
+//     forall i :: i in {e} + descendents(e) ==> match i {
+//         case Not(n) => match n {
+//             case Var(_) => true
+//             _ => false
+//         }
+//         case e => true
+//     }
+// }
 
-*/
+// function method simplify_not_expressions(e: Expression, vs: map<Variable,bool>) : (out: Expression)
+//     requires vs.Keys >= vars(e)
+//     requires no_implies(e)
+//     requires no_equivalent(out)
+//     decreases e
+//     ensures no_not_expressions(out)
+//     ensures vars(e) >= vars(out)
+//     ensures eval(e, vs) == eval(out, vs)
+// {
+//     descendents_vars(e, vs);
+//     var out := match e {
+//         case Constant(b) =>
+//             assert no_not_expressions(e);
+//             e
+//         case Var(v) =>
+//             assert no_not_expressions(e);
+//             e
+//         case Not(x) =>
+//             var xx := match x {
+//                 case Constant(b) =>
+//                     Constant(!b)
+//                 case Var(v) =>
+//                     Not(x)
+//                 case Not(xx) =>
+//                     var xxx := simplify_not_expressions(xx, vs);
+//                     xxx
+//                 case And(s) =>
+//                     var ss := set i | i in s :: simplify_not_expressions(i, vs);
+//                     assert forall i :: i in ss ==> no_not_expressions(i);
+//                     descendents_vars(e, vs);
+//                     demorgan2(ss, vs);
+//                     var xx := Or(set i | i in ss :: Not(i));
+//                     assert no_not_expressions(xx);
+//                     xx
+//                 case Or(s) =>
+//                     var ss := set i | i in s :: simplify_not_expressions(i, vs);
+//                     assert forall i :: i in ss ==> no_not_expressions(i);
+//                     descendents_vars(e, vs);
+//                     demorgan1(ss, vs);
+//                     var xx := And(set i | i in ss :: Not(i));
+//                     assert no_not_expressions(xx);
+//                     xx
+//                 case Implies(a,b) =>
+//                     assert false;
+//                     a
+//                 case Equivalent(a,b) =>
+//                     assert false;
+//                     a
+//             };
+//             assert no_not_expressions(xx);
+//             xx
+//         case And(s) =>
+//             var ss := set i | i in s :: simplify_not_expressions(i, vs);
+//             assert forall i :: i in ss ==> no_not_expressions(i);
+//             assert no_not_expressions(And(ss));
+//             And(ss)
+//         case Or(s) =>
+//             var ss := set i | i in s :: simplify_not_expressions(i, vs);
+//             assert forall i :: i in ss ==> no_not_expressions(i);
+//             assert no_not_expressions(Or(ss));
+//             Or(ss)
+//         case Implies(a,b) =>
+//             assert false;
+//             a
+//         case Equivalent(a,b) =>
+//             assert false;
+//             a
+//     };
 
+//     out
+// }
 
-
-
-
-lemma demorgan2(s: set<Expression>, vs: map<Variable,bool>)
-    requires forall i :: i in s ==> vs.Keys >= vars(i)
-    ensures eval(Not(And(s)), vs) == eval(Or(set i | i in s :: Not(i)), vs)
-{
-    var x := eval(Not(And(s)), vs);
-    var and := And(s);
-    assert eval(and, vs) == (!forall i :: i in s ==> !eval(i, vs));
-    assert x == !(!forall i :: i in s ==> !eval(i, vs));
-
-    var y := eval(Or(set i | i in s :: Not(i)), vs);
-    var nots := set i | i in s :: Not(i);
-    assert y == eval(Or(nots), vs);
-    assert eval(Or(nots), vs) == (forall i :: i in nots ==> eval(i, vs));
-    assert !(!forall i :: i in s ==> !eval(i, vs)) == (forall i :: i in s ==> eval(Not(i), vs));
-}
-
-
-
-predicate no_implies(e: Expression) {
-    forall i :: i in {e} + descendents(e) ==> match i {
-        case Implies(_,_) => false
-        case e => true
-    }
-}
-
-function method simplify_implies(e: Expression, vs: map<Variable,bool>) : (out: Expression)
-    requires vs.Keys >= vars(e)
-    decreases e
-    ensures no_implies(out)
-    ensures vars(e) >= vars(out)
-    ensures eval(e, vs) == eval(out, vs)
-{
-    descendents_vars(e, vs);
-    var out := match e {
-        case Constant(b) =>
-            assert no_implies(e);
-            e
-        case Var(v) =>
-            assert no_implies(e);
-            e
-        case Not(x) =>
-            var xx := simplify_implies(x, vs);
-            assert no_implies(xx);
-            assert no_implies(Not(xx));
-            Not(xx)
-        case And(s) =>
-            var ss := set i | i in s :: simplify_implies(i, vs);
-            assert forall i :: i in ss ==> no_implies(i);
-            assert no_implies(And(ss));
-            And(ss)
-        case Or(s) =>
-            var ss := set i | i in s :: simplify_implies(i, vs);
-            assert forall i :: i in ss ==> no_implies(i);
-            assert no_implies(Or(ss));
-            Or(ss)
-        case Implies(a,b) =>
-            var a:= simplify_implies(a, vs);
-            assert no_implies(a) && no_implies(Not(a));
-            var b := simplify_implies(b, vs);
-            assert no_implies(b);
-            assert no_implies(Or({Not(a), b}));
-            Or({Not(a), b})
-        case Equivalent(a,b) =>
-            var a:= simplify_implies(a, vs);
-            assert no_implies(a);
-            var b := simplify_implies(b, vs);
-            assert no_implies(b);
-            assert no_implies(Equivalent(a, b));
-            Equivalent(a, b)
-    };
-
-    out
-}
-
-predicate no_equivalent(e: Expression) {
-    forall i :: i in {e} + descendents(e) ==> match i {
-        case Equivalent(_,_) => false
-        case e => true
-    }
-}
-
-function method simplify_equivalent(e: Expression, vs: map<Variable,bool>) : (out: Expression)
-    requires vs.Keys >= vars(e)
-    requires no_implies(e)
-    decreases e
-    ensures no_equivalent(out)
-    ensures vars(e) >= vars(out)
-    ensures eval(e, vs) == eval(out, vs)
-{
-    descendents_vars(e, vs);
-    var out := match e {
-        case Constant(b) =>
-            assert no_equivalent(e);
-            e
-        case Var(v) =>
-            assert no_equivalent(e);
-            e
-        case Not(x) =>
-            var xx := simplify_equivalent(x, vs);
-            assert no_equivalent(xx);
-            assert no_equivalent(Not(xx));
-            Not(xx)
-        case And(s) =>
-            var ss := set i | i in s :: simplify_equivalent(i, vs);
-            assert forall i :: i in ss ==> no_equivalent(i);
-            assert no_equivalent(And(ss));
-            And(ss)
-        case Or(s) =>
-            var ss := set i | i in s :: simplify_equivalent(i, vs);
-            assert forall i :: i in ss ==> no_equivalent(i);
-            assert no_equivalent(Or(ss));
-            Or(ss)
-        case Implies(a,b) =>
-            assert false;
-            a
-        case Equivalent(a,b) =>
-            var a:= simplify_equivalent(a, vs);
-            assert no_equivalent(a);
-            var b := simplify_equivalent(b, vs);
-            assert no_equivalent(b);
-            var out := Or(And({a,b}),And({Not(a),Not(b)}));
-            assert no_implies(out);
-            out
-    };
-
-    out
-}
-
-predicate no_not_expressions(e: Expression) {
-    forall i :: i in {e} + descendents(e) ==> match i {
-        case Not(n) => match n {
-            case Var(_) => true
-            _ => false
-        }
-        case e => true
-    }
-}
-
-function method simplify_not_expressions(e: Expression, vs: map<Variable,bool>) : (out: Expression)
-    requires vs.Keys >= vars(e)
-    requires no_implies(e)
-    requires no_equivalent(out)
-    decreases e
-    ensures no_not_expressions(out)
-    ensures vars(e) >= vars(out)
-    ensures eval(e, vs) == eval(out, vs)
-{
-    descendents_vars(e, vs);
-    var out := match e {
-        case Constant(b) =>
-            assert no_not_expressions(e);
-            e
-        case Var(v) =>
-            assert no_not_expressions(e);
-            e
-        case Not(x) =>
-            var xx := match x {
-                case Constant(b) =>
-                    Constant(!b)
-                case Var(v) =>
-                    Not(x)
-                case Not(xx) =>
-                    var xxx := simplify_not_expressions(xx, vs);
-                    xxx
-                case And(s) =>
-                    var ss := set i | i in s :: simplify_not_expressions(i, vs);
-                    assert forall i :: i in ss ==> no_not_expressions(i);
-                    descendents_vars(e, vs);
-                    demorgan2(ss, vs);
-                    var xx := Or(set i | i in ss :: Not(i));
-                    assert no_not_expressions(xx);
-                    xx
-                case Or(s) =>
-                    var ss := set i | i in s :: simplify_not_expressions(i, vs);
-                    assert forall i :: i in ss ==> no_not_expressions(i);
-                    descendents_vars(e, vs);
-                    demorgan1(ss, vs);
-                    var xx := And(set i | i in ss :: Not(i));
-                    assert no_not_expressions(xx);
-                    xx
-                case Implies(a,b) =>
-                    assert false;
-                    a
-                case Equivalent(a,b) =>
-                    assert false;
-                    a
-            };
-            assert no_not_expressions(xx);
-            xx
-        case And(s) =>
-            var ss := set i | i in s :: simplify_not_expressions(i, vs);
-            assert forall i :: i in ss ==> no_not_expressions(i);
-            assert no_not_expressions(And(ss));
-            And(ss)
-        case Or(s) =>
-            var ss := set i | i in s :: simplify_not_expressions(i, vs);
-            assert forall i :: i in ss ==> no_not_expressions(i);
-            assert no_not_expressions(Or(ss));
-            Or(ss)
-        case Implies(a,b) =>
-            assert false;
-            a
-        case Equivalent(a,b) =>
-            assert false;
-            a
-    };
-
-    out
-}
-
-function method simplify(e: Expression, vs: map<Variable,bool>) : (out: Expression)
-    requires vs.Keys >= vars(e)
-    ensures no_implies(out)
-    ensures no_equivalent(out)
-{
-    var out := simplify_implies(e, vs);
-    var out := simplify_equivalent(e, vs);
-    out
-}
+// function method simplify(e: Expression, vs: map<Variable,bool>) : (out: Expression)
+//     requires vs.Keys >= vars(e)
+//     ensures no_implies(out)
+//     ensures no_equivalent(out)
+// {
+//     var out := simplify_implies(e, vs);
+//     var out := simplify_equivalent(e, vs);
+//     out
+// }
